\begin{frame}{Quiz B --- bonus question}
	\begin{align*}
		\action<+->{ \sum_{i=M}^N \sum_{j=M}^N (i+j)(i-j) }
			\action<+->{ &= \sum_{i=M}^N \sum_{j=M}^N \left( i^2 + ij - ij - j^2 \right) \\ }
			\action<+->{ &= \sum_{i=M}^N \sum_{j=M}^N \left( i^2 - j^2 \right) \\ }
			\action<+->{ &= \left( \sum_{i=M}^N \sum_{j=M}^N i^2 \right) - \left( \sum_{i=M}^N \sum_{j=M}^N j^2 \right) \\ }
			\action<+->{ &= (N-M+1) \left( \sum_{i=M}^N i^2 \right) - (N-M+1) \left( \sum_{j=M}^N j^2 \right) \\ }
			\action<+->{ &= (N-M+1) \left( \sum_{i=M}^N i^2 - \sum_{j=M}^N j^2 \right) = 0 }
	\end{align*}
\end{frame}
